atomic_heap_lang/lang.v
@@ -1,0 +1,657 @@
+From iris.program_logic Require Export language.
+From atomic_block Require Export atomic_ectx_language atomic_ectxi_language.
+From iris.algebra Require Export ofe.
+From stdpp Require Export strings.
+From stdpp Require Import gmap.
+Set Default Proof Using "Type".
+
+(** atomic_heap_lang. A version of the language heap_lang provided
+with iris featuring atomic blocks. The following is the description of
+heap_lang from the Iris development.
+
+A fairly simple language used for common Iris examples.
+
+- This is a right-to-left evaluated language, like CakeML and OCaml.
+  The reason for this is that it makes curried functions usable: Given
+  a WP for [f a b], we know that any effects [f] might have to not
+  matter until after *both* [a] and [b] are evaluated.  With
+  left-to-right evaluation, that triple is basically useless unless
+  the user let-expands [b].
+
+- For prophecy variables, we annotate the reduction steps with an
+  "observation" and tweak adequacy such that WP knows all future
+  observations.  There is another possible choice: Use
+  non-deterministic choice when creating a prophecy variable
+  ([NewProph]), and when resolving it ([ResolveProph]) make the
+  program diverge unless the variable matches.  That, however,
+  requires an erasure proof that this endless loop does not make
+  specifications useless.
+
+*)
+
+Delimit Scope expr_scope with E.
+Delimit Scope val_scope with V.
+
+Module heap_lang.
+Open Scope Z_scope.
+
+(** Expressions and vals. *)
+Definition loc := positive. (* Really, any countable type. *)
+Definition proph_id := positive.
+
+Inductive base_lit : Set :=
+  | LitInt (n : Z) | LitBool (b : bool) | LitUnit
+  | LitLoc (l : loc) | LitProphecy (p: proph_id).
+Inductive un_op : Set :=
+  | NegOp | MinusUnOp.
+Inductive bin_op : Set :=
+  | PlusOp | MinusOp | MultOp | QuotOp | RemOp (* Arithmetic *)
+  | AndOp | OrOp | XorOp (* Bitwise *)
+  | ShiftLOp | ShiftROp (* Shifts *)
+  | LeOp | LtOp | EqOp. (* Relations *)
+
+Inductive binder := BAnon | BNamed : string → binder.
+Delimit Scope binder_scope with bind.
+Bind Scope binder_scope with binder.
+Definition cons_binder (mx : binder) (X : list string) : list string :=
+  match mx with BAnon => X | BNamed x => x :: X end.
+Infix ":b:" := cons_binder (at level 60, right associativity).
+Instance binder_eq_dec_eq : EqDecision binder.
+Proof. solve_decision. Defined.
+
+Instance set_unfold_cons_binder x mx X P :
+  SetUnfold (x ∈ X) P → SetUnfold (x ∈ mx :b: X) (BNamed x = mx ∨ P).
+Proof.
+  constructor. rewrite -(set_unfold (x ∈ X) P).
+  destruct mx; rewrite /= ?elem_of_cons; naive_solver.
+Qed.
+
+Inductive expr :=
+  (* Values *)
+  | Val (v : val)
+  (* Base lambda calculus *)
+  | Var (x : string)
+  | Rec (f x : binder) (e : expr)
+  | App (e1 e2 : expr)
+  (* Base types and their operations *)
+  | UnOp (op : un_op) (e : expr)
+  | BinOp (op : bin_op) (e1 e2 : expr)
+  | If (e0 e1 e2 : expr)
+  (* Products *)
+  | Pair (e1 e2 : expr)
+  | Fst (e : expr)
+  | Snd (e : expr)
+  (* Sums *)
+  | InjL (e : expr)
+  | InjR (e : expr)
+  | Case (e0 : expr) (e1 : expr) (e2 : expr)
+  (* Concurrency *)
+  | Fork (e : expr)
+  (* Heap *)
+  | Alloc (e : expr)
+  | Load (e : expr)
+  | Store (e1 : expr) (e2 : expr)
+  | CAS (e0 : expr) (e1 : expr) (e2 : expr)
+  | FAA (e1 : expr) (e2 : expr)
+  (* Prophecy *)
+  | NewProph
+  | ResolveProph (e1 : expr) (e2 : expr)
+  (* Atomic Blocks *)
+  | AtomicBlock (e : expr)
+with val :=
+  | LitV (l : base_lit)
+  | RecV (f x : binder) (e : expr)
+  | PairV (v1 v2 : val)
+  | InjLV (v : val)
+  | InjRV (v : val).
+
+Bind Scope expr_scope with expr.
+Bind Scope val_scope with val.
+
+Definition observation : Set := proph_id * val.
+
+Notation of_val := Val (only parsing).
+
+Definition to_val (e : expr) : option val :=
+  match e with
+  | Val v => Some v
+  | _ => None
+  end.
+
+(** We assume the following encoding of values to 64-bit words: The least 3
+significant bits of every word are a "tag", and we have 61 bits of payload,
+which is enough if all pointers are 8-byte-aligned (common on 64bit
+architectures). The tags have the following meaning:
+
+0: Payload is the data for a LitV (LitInt _).
+1: Payload is the data for a InjLV (LitV (LitInt _)).
+2: Payload is the data for a InjRV (LitV (LitInt _)).
+3: Payload is the data for a LitV (LitLoc _).
+4: Payload is the data for a InjLV (LitV (LitLoc _)).
+4: Payload is the data for a InjRV (LitV (LitLoc _)).
+6: Payload is one of the following finitely many values, which 61 bits are more
+   than enough to encode:
+   LitV LitUnit, InjLV (LitV LitUnit), InjRV (LitV LitUnit),
+   LitV (LitBool _), InjLV (LitV (LitBool _)), InjRV (LitV (LitBool _)).
+7: Value is boxed, i.e., payload is a pointer to some read-only memory area on
+   the heap which stores whether this is a RecV, PairV, InjLV or InjRV and the
+   relevant data for those cases. However, the boxed representation is never
+   used if any of the above representations could be used.
+
+Ignoring (as usual) the fact that we have to fit the infinite Z/loc into 61
+bits, this means every value is machine-word-sized and can hence be atomically
+read and written.  Also notice that the sets of boxed and unboxed values are
+disjoint. *)
+Definition val_is_unboxed (v : val) : Prop :=
+  match v with
+  | LitV _ => True
+  | InjLV (LitV _) => True
+  | InjRV (LitV _) => True
+  | _ => False
+  end.
+
+(** The state: heaps of vals. *)
+Record state : Type := {
+  heap: gmap loc val;
+  used_proph_id: gset proph_id;
+}.
+
+(** Equality and other typeclass stuff *)
+Lemma to_of_val v : to_val (of_val v) = Some v.
+Proof. by destruct v. Qed.
+
+Lemma of_to_val e v : to_val e = Some v → of_val v = e.
+Proof. destruct e=>//=. by intros [= <-]. Qed.
+
+Instance of_val_inj : Inj (=) (=) of_val.
+Proof. intros ??. congruence. Qed.
+
+Instance base_lit_eq_dec : EqDecision base_lit.
+Proof. solve_decision. Defined.
+Instance un_op_eq_dec : EqDecision un_op.
+Proof. solve_decision. Defined.
+Instance bin_op_eq_dec : EqDecision bin_op.
+Proof. solve_decision. Defined.
+Instance expr_eq_dec : EqDecision expr.
+Proof.
+  refine (
+   fix go (e1 e2 : expr) {struct e1} : Decision (e1 = e2) :=
+     match e1, e2 with
+     | Val v, Val v' => cast_if (decide (v = v'))
+     | Var x, Var x' => cast_if (decide (x = x'))
+     | Rec f x e, Rec f' x' e' =>
+        cast_if_and3 (decide (f = f')) (decide (x = x')) (decide (e = e'))
+     | App e1 e2, App e1' e2' => cast_if_and (decide (e1 = e1')) (decide (e2 = e2'))
+     | UnOp o e, UnOp o' e' => cast_if_and (decide (o = o')) (decide (e = e'))
+     | BinOp o e1 e2, BinOp o' e1' e2' =>
+        cast_if_and3 (decide (o = o')) (decide (e1 = e1')) (decide (e2 = e2'))
+     | If e0 e1 e2, If e0' e1' e2' =>
+        cast_if_and3 (decide (e0 = e0')) (decide (e1 = e1')) (decide (e2 = e2'))
+     | Pair e1 e2, Pair e1' e2' =>
+        cast_if_and (decide (e1 = e1')) (decide (e2 = e2'))
+     | Fst e, Fst e' => cast_if (decide (e = e'))
+     | Snd e, Snd e' => cast_if (decide (e = e'))
+     | InjL e, InjL e' => cast_if (decide (e = e'))
+     | InjR e, InjR e' => cast_if (decide (e = e'))
+     | Case e0 e1 e2, Case e0' e1' e2' =>
+        cast_if_and3 (decide (e0 = e0')) (decide (e1 = e1')) (decide (e2 = e2'))
+     | Fork e, Fork e' => cast_if (decide (e = e'))
+     | Alloc e, Alloc e' => cast_if (decide (e = e'))
+     | Load e, Load e' => cast_if (decide (e = e'))
+     | Store e1 e2, Store e1' e2' =>
+        cast_if_and (decide (e1 = e1')) (decide (e2 = e2'))
+     | CAS e0 e1 e2, CAS e0' e1' e2' =>
+        cast_if_and3 (decide (e0 = e0')) (decide (e1 = e1')) (decide (e2 = e2'))
+     | FAA e1 e2, FAA e1' e2' =>
+        cast_if_and (decide (e1 = e1')) (decide (e2 = e2'))
+     | NewProph, NewProph => left _
+     | ResolveProph e1 e2, ResolveProph e1' e2' =>
+        cast_if_and (decide (e1 = e1')) (decide (e2 = e2'))
+     | AtomicBlock e, AtomicBlock e' => cast_if (decide (e = e'))
+     | _, _ => right _
+     end
+   with gov (v1 v2 : val) {struct v1} : Decision (v1 = v2) :=
+     match v1, v2 with
+     | LitV l, LitV l' => cast_if (decide (l = l'))
+     | RecV f x e, RecV f' x' e' =>
+        cast_if_and3 (decide (f = f')) (decide (x = x')) (decide (e = e'))
+     | PairV e1 e2, PairV e1' e2' =>
+        cast_if_and (decide (e1 = e1')) (decide (e2 = e2'))
+     | InjLV e, InjLV e' => cast_if (decide (e = e'))
+     | InjRV e, InjRV e' => cast_if (decide (e = e'))
+     | _, _ => right _
+     end
+   for go); try (clear go gov; abstract intuition congruence).
+Defined.
+Instance val_eq_dec : EqDecision val.
+Proof. solve_decision. Defined.
+
+Instance base_lit_countable : Countable base_lit.
+Proof.
+ refine (inj_countable' (λ l, match l with
+  | LitInt n => (inl (inl n), None) | LitBool b => (inl (inr b), None)
+  | LitUnit => (inr (inl ()), None) | LitLoc l => (inr (inr l), None)
+  | LitProphecy p => (inr (inl ()), Some p)
+  end) (λ l, match l with
+  | (inl (inl n), None) => LitInt n | (inl (inr b), None) => LitBool b
+  | (inr (inl ()), None) => LitUnit | (inr (inr l), None) => LitLoc l
+  | (_, Some p) => LitProphecy p
+  end) _); by intros [].
+Qed.
+Instance un_op_finite : Countable un_op.
+Proof.
+ refine (inj_countable' (λ op, match op with NegOp => 0 | MinusUnOp => 1 end)
+  (λ n, match n with 0 => NegOp | _ => MinusUnOp end) _); by intros [].
+Qed.
+Instance bin_op_countable : Countable bin_op.
+Proof.
+ refine (inj_countable' (λ op, match op with
+  | PlusOp => 0 | MinusOp => 1 | MultOp => 2 | QuotOp => 3 | RemOp => 4
+  | AndOp => 5 | OrOp => 6 | XorOp => 7 | ShiftLOp => 8 | ShiftROp => 9
+  | LeOp => 10 | LtOp => 11 | EqOp => 12
+  end) (λ n, match n with
+  | 0 => PlusOp | 1 => MinusOp | 2 => MultOp | 3 => QuotOp | 4 => RemOp
+  | 5 => AndOp | 6 => OrOp | 7 => XorOp | 8 => ShiftLOp | 9 => ShiftROp
+  | 10 => LeOp | 11 => LtOp | _ => EqOp
+  end) _); by intros [].
+Qed.
+Instance binder_countable : Countable binder.
+Proof.
+ refine (inj_countable' (λ b, match b with BNamed s => Some s | BAnon => None end)
+  (λ b, match b with Some s => BNamed s | None => BAnon end) _); by intros [].
+Qed.
+Instance expr_countable : Countable expr.
+Proof.
+ set (enc :=
+   fix go e :=
+     match e with
+     | Val v => GenNode 0 [gov v]
+     | Var x => GenLeaf (inl (inl x))
+     | Rec f x e => GenNode 1 [GenLeaf (inl (inr f)); GenLeaf (inl (inr x)); go e]
+     | App e1 e2 => GenNode 2 [go e1; go e2]
+     | UnOp op e => GenNode 3 [GenLeaf (inr (inr (inl op))); go e]
+     | BinOp op e1 e2 => GenNode 4 [GenLeaf (inr (inr (inr op))); go e1; go e2]
+     | If e0 e1 e2 => GenNode 5 [go e0; go e1; go e2]
+     | Pair e1 e2 => GenNode 6 [go e1; go e2]
+     | Fst e => GenNode 7 [go e]
+     | Snd e => GenNode 8 [go e]
+     | InjL e => GenNode 9 [go e]
+     | InjR e => GenNode 10 [go e]
+     | Case e0 e1 e2 => GenNode 11 [go e0; go e1; go e2]
+     | Fork e => GenNode 12 [go e]
+     | Alloc e => GenNode 13 [go e]
+     | Load e => GenNode 14 [go e]
+     | Store e1 e2 => GenNode 15 [go e1; go e2]
+     | CAS e0 e1 e2 => GenNode 16 [go e0; go e1; go e2]
+     | FAA e1 e2 => GenNode 17 [go e1; go e2]
+     | NewProph => GenNode 18 []
+     | ResolveProph e1 e2 => GenNode 19 [go e1; go e2]
+     | AtomicBlock e => GenNode 20 [go e]
+     end
+   with gov v :=
+     match v with
+     | LitV l => GenLeaf (inr (inl l))
+     | RecV f x e =>
+        GenNode 0 [GenLeaf (inl (inr f)); GenLeaf (inl (inr x)); go e]
+     | PairV v1 v2 => GenNode 1 [gov v1; gov v2]
+     | InjLV v => GenNode 2 [gov v]
+     | InjRV v => GenNode 3 [gov v]
+     end
+   for go).
+ set (dec :=
+   fix go e :=
+     match e with
+     | GenNode 0 [v] => Val (gov v)
+     | GenLeaf (inl (inl x)) => Var x
+     | GenNode 1 [GenLeaf (inl (inr f)); GenLeaf (inl (inr x)); e] => Rec f x (go e)
+     | GenNode 2 [e1; e2] => App (go e1) (go e2)
+     | GenNode 3 [GenLeaf (inr (inr (inl op))); e] => UnOp op (go e)
+     | GenNode 4 [GenLeaf (inr (inr (inr op))); e1; e2] => BinOp op (go e1) (go e2)
+     | GenNode 5 [e0; e1; e2] => If (go e0) (go e1) (go e2)
+     | GenNode 6 [e1; e2] => Pair (go e1) (go e2)
+     | GenNode 7 [e] => Fst (go e)
+     | GenNode 8 [e] => Snd (go e)
+     | GenNode 9 [e] => InjL (go e)
+     | GenNode 10 [e] => InjR (go e)
+     | GenNode 11 [e0; e1; e2] => Case (go e0) (go e1) (go e2)
+     | GenNode 12 [e] => Fork (go e)
+     | GenNode 13 [e] => Alloc (go e)
+     | GenNode 14 [e] => Load (go e)
+     | GenNode 15 [e1; e2] => Store (go e1) (go e2)
+     | GenNode 16 [e0; e1; e2] => CAS (go e0) (go e1) (go e2)
+     | GenNode 17 [e1; e2] => FAA (go e1) (go e2)
+     | GenNode 18 [] => NewProph
+     | GenNode 19 [e1; e2] => ResolveProph (go e1) (go e2)
+     | GenNode 20 [e] => AtomicBlock (go e)
+     | _ => Val $ LitV LitUnit (* dummy *)
+     end
+   with gov v :=
+     match v with
+     | GenLeaf (inr (inl l)) => LitV l
+     | GenNode 0 [GenLeaf (inl (inr f)); GenLeaf (inl (inr x)); e] => RecV f x (go e)
+     | GenNode 1 [v1; v2] => PairV (gov v1) (gov v2)
+     | GenNode 2 [v] => InjLV (gov v)
+     | GenNode 3 [v] => InjRV (gov v)
+     | _ => LitV LitUnit (* dummy *)
+     end
+   for go).
+ refine (inj_countable' enc dec _).
+ refine (fix go (e : expr) {struct e} := _ with gov (v : val) {struct v} := _ for go).
+ - destruct e as [v| | | | | | | | | | | | | | | | | | | | |]; simpl; f_equal;
+     [exact (gov v)|done..].
+ - destruct v; by f_equal.
+Qed.
+Instance val_countable : Countable val.
+Proof. refine (inj_countable of_val to_val _); auto using to_of_val. Qed.
+
+Instance state_inhabited : Inhabited state :=
+  populate {| heap := inhabitant; used_proph_id := inhabitant |}.
+Instance val_inhabited : Inhabited val := populate (LitV LitUnit).
+Instance expr_inhabited : Inhabited expr := populate (Val inhabitant).
+
+Canonical Structure stateC := leibnizC state.
+Canonical Structure locC := leibnizC loc.
+Canonical Structure valC := leibnizC val.
+Canonical Structure exprC := leibnizC expr.
+
+(** Evaluation contexts *)
+Inductive ectx_item :=
+  | AppLCtx (v2 : val)
+  | AppRCtx (e1 : expr)
+  | UnOpCtx (op : un_op)
+  | BinOpLCtx (op : bin_op) (v2 : val)
+  | BinOpRCtx (op : bin_op) (e1 : expr)
+  | IfCtx (e1 e2 : expr)
+  | PairLCtx (v2 : val)
+  | PairRCtx (e1 : expr)
+  | FstCtx
+  | SndCtx
+  | InjLCtx
+  | InjRCtx
+  | CaseCtx (e1 : expr) (e2 : expr)
+  | AllocCtx
+  | LoadCtx
+  | StoreLCtx (v2 : val)
+  | StoreRCtx (e1 : expr)
+  | CasLCtx (v1 : val) (v2 : val)
+  | CasMCtx (e0 : expr) (v2 : val)
+  | CasRCtx (e0 : expr) (e1 : expr)
+  | FaaLCtx (v2 : val)
+  | FaaRCtx (e1 : expr)
+  | ProphLCtx (v2 : val)
+  | ProphRCtx (e1 : expr).
+
+Definition fill_item (Ki : ectx_item) (e : expr) : expr :=
+  match Ki with
+  | AppLCtx v2 => App e (of_val v2)
+  | AppRCtx e1 => App e1 e
+  | UnOpCtx op => UnOp op e
+  | BinOpLCtx op v2 => BinOp op e (Val v2)
+  | BinOpRCtx op e1 => BinOp op e1 e
+  | IfCtx e1 e2 => If e e1 e2
+  | PairLCtx v2 => Pair e (Val v2)
+  | PairRCtx e1 => Pair e1 e
+  | FstCtx => Fst e
+  | SndCtx => Snd e
+  | InjLCtx => InjL e
+  | InjRCtx => InjR e
+  | CaseCtx e1 e2 => Case e e1 e2
+  | AllocCtx => Alloc e
+  | LoadCtx => Load e
+  | StoreLCtx v2 => Store e (Val v2)
+  | StoreRCtx e1 => Store e1 e
+  | CasLCtx v1 v2 => CAS e (Val v1) (Val v2)
+  | CasMCtx e0 v2 => CAS e0 e (Val v2)
+  | CasRCtx e0 e1 => CAS e0 e1 e
+  | FaaLCtx v2 => FAA e (Val v2)
+  | FaaRCtx e1 => FAA e1 e
+  | ProphLCtx v2 => ResolveProph e (of_val v2)
+  | ProphRCtx e1 => ResolveProph e1 e
+  end.
+
+(** Substitution *)
+Fixpoint subst (x : string) (v : val) (e : expr)  : expr :=
+  match e with
+  | Val _ => e
+  | Var y => if decide (x = y) then Val v else Var y
+  | Rec f y e =>
+     Rec f y $ if decide (BNamed x ≠ f ∧ BNamed x ≠ y) then subst x v e else e
+  | App e1 e2 => App (subst x v e1) (subst x v e2)
+  | UnOp op e => UnOp op (subst x v e)
+  | BinOp op e1 e2 => BinOp op (subst x v e1) (subst x v e2)
+  | If e0 e1 e2 => If (subst x v e0) (subst x v e1) (subst x v e2)
+  | Pair e1 e2 => Pair (subst x v e1) (subst x v e2)
+  | Fst e => Fst (subst x v e)
+  | Snd e => Snd (subst x v e)
+  | InjL e => InjL (subst x v e)
+  | InjR e => InjR (subst x v e)
+  | Case e0 e1 e2 => Case (subst x v e0) (subst x v e1) (subst x v e2)
+  | Fork e => Fork (subst x v e)
+  | Alloc e => Alloc (subst x v e)
+  | Load e => Load (subst x v e)
+  | Store e1 e2 => Store (subst x v e1) (subst x v e2)
+  | CAS e0 e1 e2 => CAS (subst x v e0) (subst x v e1) (subst x v e2)
+  | FAA e1 e2 => FAA (subst x v e1) (subst x v e2)
+  | NewProph => NewProph
+  | ResolveProph e1 e2 => ResolveProph (subst x v e1) (subst x v e2)
+  | AtomicBlock e => AtomicBlock (subst x v e)
+  end.
+
+Definition subst' (mx : binder) (v : val) : expr → expr :=
+  match mx with BNamed x => subst x v | BAnon => id end.
+
+(** The stepping relation *)
+Definition un_op_eval (op : un_op) (v : val) : option val :=
+  match op, v with
+  | NegOp, LitV (LitBool b) => Some $ LitV $ LitBool (negb b)
+  | NegOp, LitV (LitInt n) => Some $ LitV $ LitInt (Z.lnot n)
+  | MinusUnOp, LitV (LitInt n) => Some $ LitV $ LitInt (- n)
+  | _, _ => None
+  end.
+
+Definition bin_op_eval_int (op : bin_op) (n1 n2 : Z) : base_lit :=
+  match op with
+  | PlusOp => LitInt (n1 + n2)
+  | MinusOp => LitInt (n1 - n2)
+  | MultOp => LitInt (n1 * n2)
+  | QuotOp => LitInt (n1 `quot` n2)
+  | RemOp => LitInt (n1 `rem` n2)
+  | AndOp => LitInt (Z.land n1 n2)
+  | OrOp => LitInt (Z.lor n1 n2)
+  | XorOp => LitInt (Z.lxor n1 n2)
+  | ShiftLOp => LitInt (n1 ≪ n2)
+  | ShiftROp => LitInt (n1 ≫ n2)
+  | LeOp => LitBool (bool_decide (n1 ≤ n2))
+  | LtOp => LitBool (bool_decide (n1 < n2))
+  | EqOp => LitBool (bool_decide (n1 = n2))
+  end.
+
+Definition bin_op_eval_bool (op : bin_op) (b1 b2 : bool) : option base_lit :=
+  match op with
+  | PlusOp | MinusOp | MultOp | QuotOp | RemOp => None (* Arithmetic *)
+  | AndOp => Some (LitBool (b1 && b2))
+  | OrOp => Some (LitBool (b1 || b2))
+  | XorOp => Some (LitBool (xorb b1 b2))
+  | ShiftLOp | ShiftROp => None (* Shifts *)
+  | LeOp | LtOp => None (* InEquality *)
+  | EqOp => Some (LitBool (bool_decide (b1 = b2)))
+  end.
+
+Definition bin_op_eval (op : bin_op) (v1 v2 : val) : option val :=
+  if decide (op = EqOp) then Some $ LitV $ LitBool $ bool_decide (v1 = v2) else
+  match v1, v2 with
+  | LitV (LitInt n1), LitV (LitInt n2) => Some $ LitV $ bin_op_eval_int op n1 n2
+  | LitV (LitBool b1), LitV (LitBool b2) => LitV <$> bin_op_eval_bool op b1 b2
+  | _, _ => None
+  end.
+
+(** CAS just compares the word-sized representation of the two values, it cannot
+look into boxed data.  This works out fine if at least one of the to-be-compared
+values is unboxed (exploiting the fact that an unboxed and a boxed value can
+never be equal because these are disjoint sets).  *)
+Definition vals_cas_compare_safe (vl v1 : val) : Prop :=
+  val_is_unboxed vl ∨ val_is_unboxed v1.
+Arguments vals_cas_compare_safe !_ !_ /.
+
+Definition state_upd_heap (f: gmap loc val → gmap loc val) (σ: state) : state :=
+  {| heap := f σ.(heap); used_proph_id := σ.(used_proph_id) |}.
+Arguments state_upd_heap _ !_ /.
+Definition state_upd_used_proph_id (f: gset proph_id → gset proph_id) (σ: state) : state :=
+  {| heap := σ.(heap); used_proph_id := f σ.(used_proph_id) |}.
+Arguments state_upd_used_proph_id _ !_ /.
+
+Inductive head_step : expr → state → list observation → expr → state → list (expr) → Prop :=
+  | RecS f x e σ :
+     head_step (Rec f x e) σ [] (Val $ RecV f x e) σ []
+  | PairS v1 v2 σ :
+     head_step (Pair (Val v1) (Val v2)) σ [] (Val $ PairV v1 v2) σ []
+  | InjLS v σ :
+     head_step (InjL $ Val v) σ [] (Val $ InjLV v) σ []
+  | InjRS v σ :
+     head_step (InjR $ Val v) σ [] (Val $ InjRV v) σ []
+  | BetaS f x e1 v2 e' σ :
+     e' = subst' x v2 (subst' f (RecV f x e1) e1) →
+     head_step (App (Val $ RecV f x e1) (Val v2)) σ [] e' σ []
+  | UnOpS op v v' σ :
+     un_op_eval op v = Some v' →
+     head_step (UnOp op (Val v)) σ [] (Val v') σ []
+  | BinOpS op v1 v2 v' σ :
+     bin_op_eval op v1 v2 = Some v' →
+     head_step (BinOp op (Val v1) (Val v2)) σ [] (Val v') σ []
+  | IfTrueS e1 e2 σ :
+     head_step (If (Val $ LitV $ LitBool true) e1 e2) σ [] e1 σ []
+  | IfFalseS e1 e2 σ :
+     head_step (If (Val $ LitV $ LitBool false) e1 e2) σ [] e2 σ []
+  | FstS v1 v2 σ :
+     head_step (Fst (Val $ PairV v1 v2)) σ [] (Val v1) σ []
+  | SndS v1 v2 σ :
+     head_step (Snd (Val $ PairV v1 v2)) σ [] (Val v2) σ []
+  | CaseLS v e1 e2 σ :
+     head_step (Case (Val $ InjLV v) e1 e2) σ [] (App e1 (Val v)) σ []
+  | CaseRS v e1 e2 σ :
+     head_step (Case (Val $ InjRV v) e1 e2) σ [] (App e2 (Val v)) σ []
+  | ForkS e σ:
+     head_step (Fork e) σ [] (Val $ LitV LitUnit) σ [e]
+  | AllocS v σ l :
+     σ.(heap) !! l = None →
+     head_step (Alloc $ Val v) σ
+               []
+               (Val $ LitV $ LitLoc l) (state_upd_heap <[l:=v]> σ)
+               []
+  | LoadS l v σ :
+     σ.(heap) !! l = Some v →
+     head_step (Load (Val $ LitV $ LitLoc l)) σ [] (of_val v) σ []
+  | StoreS l v σ :
+     is_Some (σ.(heap) !! l) →
+     head_step (Store (Val $ LitV $ LitLoc l) (Val v)) σ
+               []
+               (Val $ LitV LitUnit) (state_upd_heap <[l:=v]> σ)
+               []
+  | CasFailS l v1 v2 vl σ :
+     σ.(heap) !! l = Some vl → vl ≠ v1 →
+     vals_cas_compare_safe vl v1 →
+     head_step (CAS (Val $ LitV $ LitLoc l) (Val v1) (Val v2)) σ []
+               (Val $ LitV $ LitBool false) σ []
+  | CasSucS l v1 v2 σ :
+     σ.(heap) !! l = Some v1 →
+     vals_cas_compare_safe v1 v1 →
+     head_step (CAS (Val $ LitV $ LitLoc l) (Val v1) (Val v2)) σ
+               []
+               (Val $ LitV $ LitBool true) (state_upd_heap <[l:=v2]> σ)
+               []
+  | FaaS l i1 i2 σ :
+     σ.(heap) !! l = Some (LitV (LitInt i1)) →
+     head_step (FAA (Val $ LitV $ LitLoc l) (Val $ LitV $ LitInt i2)) σ
+               []
+               (Val $ LitV $ LitInt i1) (state_upd_heap <[l:=LitV (LitInt (i1 + i2))]>σ)
+               []
+  | NewProphS σ p :
+     p ∉ σ.(used_proph_id) →
+     head_step NewProph σ
+               []
+               (Val $ LitV $ LitProphecy p) (state_upd_used_proph_id ({[ p ]} ∪) σ)
+               []
+  | ResolveProphS e1 p e2 v σ :
+     to_val e1 = Some (LitV $ LitProphecy p) →
+     to_val e2 = Some v →
+     head_step (ResolveProph (Val $ LitV $ LitProphecy p) (Val v)) σ
+               [(p, v)]
+               (Val $ LitV LitUnit) σ [].
+
+(** Basic properties about the language *)
+Instance fill_item_inj Ki : Inj (=) (=) (fill_item Ki).
+Proof. destruct Ki; intros ???; simplify_eq/=; auto with f_equal. Qed.
+
+Lemma fill_item_val Ki e :
+  is_Some (to_val (fill_item Ki e)) → is_Some (to_val e).
+Proof. intros [v ?]. destruct Ki; simplify_option_eq; eauto. Qed.
+
+Lemma val_head_stuck e1 σ1 κ e2 σ2 efs : head_step e1 σ1 κ e2 σ2 efs → to_val e1 = None.
+Proof. destruct 1; naive_solver. Qed.
+
+Lemma head_ctx_step_val Ki e σ1 κ e2 σ2 efs :
+  head_step (fill_item Ki e) σ1 κ e2 σ2 efs → is_Some (to_val e).
+Proof. destruct Ki; inversion_clear 1; simplify_option_eq; by eauto. Qed.
+
+Lemma fill_item_no_val_inj Ki1 Ki2 e1 e2 :
+  to_val e1 = None → to_val e2 = None →
+  fill_item Ki1 e1 = fill_item Ki2 e2 → Ki1 = Ki2.
+Proof. destruct Ki1, Ki2; intros; by simplify_eq. Qed.
+
+Lemma alloc_fresh v σ :
+  let l := fresh (dom (gset loc) σ.(heap)) in
+  head_step (Alloc $ Val v) σ [] (Val $ LitV $ LitLoc l) (state_upd_heap <[l:=v]> σ) [].
+Proof. by intros; apply AllocS, (not_elem_of_dom (D:=gset loc)), is_fresh. Qed.
+
+Lemma new_proph_id_fresh σ :
+  let p := fresh σ.(used_proph_id) in
+  head_step NewProph σ [] (Val $ LitV $ LitProphecy p) (state_upd_used_proph_id ({[ p ]} ∪) σ) [].
+Proof. constructor. apply is_fresh. Qed.
+
+Definition atomic_block_of (e : expr) :=
+  match e with
+  | AtomicBlock ab => Some ab
+  | _ => None
+  end.
+
+Lemma atomic_block_head_stuck e1 σ1 κ e2 σ2 efs :
+  head_step e1 σ1 κ e2 σ2 efs → atomic_block_of e1 = None.
+Proof. destruct e1; auto; inversion 1. Qed.
+Lemma atomic_block_not_val e ab : atomic_block_of e = Some ab → to_val e = None.
+Proof. by destruct e. Qed.
+Lemma atomic_block_no_ectx e ae :
+  atomic_block_of e = Some ae → ∀ (Ki : ectx_item) (e' : expr), e ≠ fill_item Ki e'.
+Proof.
+  destruct e; inversion 1; simplify_eq.
+  intros Ki e'; by destruct Ki; simpl.
+Qed.
+
+Lemma heap_lang_mixin :
+  AtomicEctxiLanguageMixin of_val to_val atomic_block_of fill_item head_step.
+Proof.
+  split; apply _ || eauto using to_of_val, of_to_val, val_head_stuck,
+    fill_item_val, fill_item_no_val_inj, head_ctx_step_val,
+    atomic_block_head_stuck, atomic_block_not_val, atomic_block_no_ectx.
+Qed.
+End heap_lang.
+
+(** Language *)
+Canonical Structure heap_ectxi_lang := AtomicEctxiLanguage heap_lang.heap_lang_mixin.
+Canonical Structure heap_ectx_lang := AtomicEctxLanguageOfEctxi heap_ectxi_lang.
+Canonical Structure heap_lang := AtomicLanguageOfEctx heap_ectx_lang.
+
+(* Prefer heap_lang names over ectx_language names. *)
+Export heap_lang.
+
+(** Define some derived forms. *)
+Notation Lam x e := (Rec BAnon x e) (only parsing).
+Notation Let x e1 e2 := (App (Lam x e2) e1) (only parsing).
+Notation Seq e1 e2 := (Let BAnon e1 e2) (only parsing).
+Notation LamV x e := (RecV BAnon x e) (only parsing).
+Notation LetCtx x e2 := (AppRCtx (LamV x e2)) (only parsing).
+Notation SeqCtx e2 := (LetCtx BAnon e2) (only parsing).
+Notation Match e0 x1 e1 x2 e2 := (Case e0 (Lam x1 e1) (Lam x2 e2)) (only parsing).
+
+(* Skip should be atomic, we sometimes open invariants around
+   it. Hence, we need to explicitly use LamV instead of e.g., Seq. *)
+Notation Skip := (App (Val $ LamV BAnon (Val $ LitV LitUnit)) (Val $ LitV LitUnit)).
