atomic_heap_lang/metatheory.v
@@ -1,0 +1,190 @@
+From atomic_block.atomic_heap_lang Require Export lang.
+From stdpp Require Import gmap.
+
+(* This file contains some metatheory about the heap_lang language,
+  which is not needed for verifying programs. *)
+
+(* Closed expressions and values. *)
+Fixpoint is_closed_expr (X : list string) (e : expr) : bool :=
+  match e with
+  | Val v => is_closed_val v
+  | Var x => bool_decide (x ∈ X)
+  | Rec f x e => is_closed_expr (f :b: x :b: X) e
+  | UnOp _ e | Fst e | Snd e | InjL e | InjR e | Fork e | Alloc e | Load e =>
+     is_closed_expr X e
+  | App e1 e2 | BinOp _ e1 e2 | Pair e1 e2 | Store e1 e2 | FAA e1 e2
+  | ResolveProph e1 e2 =>
+     is_closed_expr X e1 && is_closed_expr X e2
+  | If e0 e1 e2 | Case e0 e1 e2 | CAS e0 e1 e2 =>
+     is_closed_expr X e0 && is_closed_expr X e1 && is_closed_expr X e2
+  | NewProph => true
+  | AtomicBlock e => is_closed_expr X e
+  end
+with is_closed_val (v : val) : bool :=
+  match v with
+  | LitV _ => true
+  | RecV f x e => is_closed_expr (f :b: x :b: []) e
+  | PairV v1 v2 => is_closed_val v1 && is_closed_val v2
+  | InjLV v | InjRV v => is_closed_val v
+  end.
+
+Lemma is_closed_weaken X Y e : is_closed_expr X e → X ⊆ Y → is_closed_expr Y e.
+Proof. revert X Y; induction e; naive_solver (eauto; set_solver). Qed.
+
+Lemma is_closed_weaken_nil X e : is_closed_expr [] e → is_closed_expr X e.
+Proof. intros. by apply is_closed_weaken with [], list_subseteq_nil. Qed.
+
+Lemma is_closed_subst X e x v :
+  is_closed_val v → is_closed_expr (x :: X) e → is_closed_expr X (subst x v e).
+Proof.
+  intros Hv. revert X.
+  induction e=> X /= ?; destruct_and?; split_and?; simplify_option_eq;
+    try match goal with
+    | H : ¬(_ ∧ _) |- _ => apply not_and_l in H as [?%dec_stable|?%dec_stable]
+    end; eauto using is_closed_weaken with set_solver.
+Qed.
+Lemma is_closed_subst' X e x v :
+  is_closed_val v → is_closed_expr (x :b: X) e → is_closed_expr X (subst' x v e).
+Proof. destruct x; eauto using is_closed_subst. Qed.
+
+(* Substitution *)
+Lemma subst_is_closed X e x es : is_closed_expr X e → x ∉ X → subst x es e = e.
+Proof.
+  revert X. induction e=> X /=; rewrite ?bool_decide_spec ?andb_True=> ??;
+    repeat case_decide; simplify_eq/=; f_equal; intuition eauto with set_solver.
+Qed.
+
+Lemma subst_is_closed_nil e x v : is_closed_expr [] e → subst x v e = e.
+Proof. intros. apply subst_is_closed with []; set_solver. Qed.
+
+Lemma subst_subst e x v v' :
+  subst x v (subst x v' e) = subst x v' e.
+Proof.
+  intros. induction e; simpl; try (f_equal; by auto);
+    simplify_option_eq; auto using subst_is_closed_nil with f_equal.
+Qed.
+Lemma subst_subst' e x v v' :
+  subst' x v (subst' x v' e) = subst' x v' e.
+Proof. destruct x; simpl; auto using subst_subst. Qed.
+
+Lemma subst_subst_ne e x y v v' :
+  x ≠ y → subst x v (subst y v' e) = subst y v' (subst x v e).
+Proof.
+  intros. induction e; simpl; try (f_equal; by auto);
+    simplify_option_eq; auto using eq_sym, subst_is_closed_nil with f_equal.
+Qed.
+Lemma subst_subst_ne' e x y v v' :
+  x ≠ y → subst' x v (subst' y v' e) = subst' y v' (subst' x v e).
+Proof. destruct x, y; simpl; auto using subst_subst_ne with congruence. Qed.
+
+Lemma subst_rec' f y e x v :
+  x = f ∨ x = y ∨ x = BAnon →
+  subst' x v (Rec f y e) = Rec f y e.
+Proof. intros. destruct x; simplify_option_eq; naive_solver. Qed.
+Lemma subst_rec_ne' f y e x v :
+  (x ≠ f ∨ f = BAnon) → (x ≠ y ∨ y = BAnon) →
+  subst' x v (Rec f y e) = Rec f y (subst' x v e).
+Proof. intros. destruct x; simplify_option_eq; naive_solver. Qed.
+
+(* The stepping relation preserves closedness *)
+Lemma head_step_is_closed e1 σ1 obs e2 σ2 es :
+  is_closed_expr [] e1 →
+  map_Forall (λ _ v, is_closed_val v) σ1.(heap) →
+  head_step e1 σ1 obs e2 σ2 es →
+
+  is_closed_expr [] e2 ∧ Forall (is_closed_expr []) es ∧
+  map_Forall (λ _ v, is_closed_val v) σ2.(heap).
+Proof.
+  intros Cl1 Clσ1 STEP.
+  destruct STEP; simpl in *; split_and!;
+    try apply map_Forall_insert_2; try by naive_solver.
+  - subst. repeat apply is_closed_subst'; naive_solver.
+  - unfold un_op_eval in *. repeat case_match; naive_solver.
+  - unfold bin_op_eval, bin_op_eval_bool in *. repeat case_match; naive_solver.
+Qed.
+
+(* Parallel substitution with maps of values indexed by strings *)
+Definition binder_delete {A} (x : binder) (vs : gmap string A) : gmap string A :=
+  if x is BNamed x' then delete x' vs else vs.
+Definition binder_insert {A} (x : binder) (v : A) (vs : gmap string A) : gmap string A :=
+  if x is BNamed x' then <[x':=v]>vs else vs.
+
+Lemma binder_insert_fmap {A B : Type} (f : A → B) (x : A) b vs :
+  f <$> binder_insert b x vs = binder_insert b (f x) (f <$> vs).
+Proof. destruct b; rewrite ?fmap_insert //. Qed.
+Lemma lookup_binder_delete_None {A : Type} (vs : gmap string A) x y :
+  binder_delete x vs !! y = None ↔ x = BNamed y ∨ vs !! y = None.
+Proof. destruct x; rewrite /= ?lookup_delete_None; naive_solver. Qed.
+
+Fixpoint subst_map (vs : gmap string val) (e : expr) : expr :=
+  match e with
+  | Val _ => e
+  | Var y => if vs !! y is Some v then Val v else Var y
+  | Rec f y e => Rec f y (subst_map (binder_delete y (binder_delete f vs)) e)
+  | App e1 e2 => App (subst_map vs e1) (subst_map vs e2)
+  | UnOp op e => UnOp op (subst_map vs e)
+  | BinOp op e1 e2 => BinOp op (subst_map vs e1) (subst_map vs e2)
+  | If e0 e1 e2 => If (subst_map vs e0) (subst_map vs e1) (subst_map vs e2)
+  | Pair e1 e2 => Pair (subst_map vs e1) (subst_map vs e2)
+  | Fst e => Fst (subst_map vs e)
+  | Snd e => Snd (subst_map vs e)
+  | InjL e => InjL (subst_map vs e)
+  | InjR e => InjR (subst_map vs e)
+  | Case e0 e1 e2 => Case (subst_map vs e0) (subst_map vs e1) (subst_map vs e2)
+  | Fork e => Fork (subst_map vs e)
+  | Alloc e => Alloc (subst_map vs e)
+  | Load e => Load (subst_map vs e)
+  | Store e1 e2 => Store (subst_map vs e1) (subst_map vs e2)
+  | CAS e0 e1 e2 => CAS (subst_map vs e0) (subst_map vs e1) (subst_map vs e2)
+  | FAA e1 e2 => FAA (subst_map vs e1) (subst_map vs e2)
+  | NewProph => NewProph
+  | ResolveProph e1 e2 => ResolveProph (subst_map vs e1) (subst_map vs e2)
+  | AtomicBlock e => AtomicBlock (subst_map vs e)
+  end.
+
+Lemma subst_map_empty e : subst_map ∅ e = e.
+Proof.
+  assert (∀ x, binder_delete x (∅:gmap _ val) = ∅) as Hdel.
+  { intros [|x]; by rewrite /= ?delete_empty. }
+  induction e; simplify_map_eq; rewrite ?Hdel; auto with f_equal.
+Qed.
+Lemma subst_map_insert x v vs e :
+  subst_map (<[x:=v]>vs) e = subst x v (subst_map (delete x vs) e).
+Proof.
+  revert vs. assert (∀ (y : binder) (vs : gmap _ val), y ≠ BNamed x →
+    binder_delete y (<[x:=v]> vs) = <[x:=v]> (binder_delete y vs)) as Hins.
+  { intros [|y] vs ?; rewrite /= ?delete_insert_ne //; congruence. }
+  assert (∀ (y : binder) (vs : gmap _ val),
+    binder_delete y (delete x vs) = delete x (binder_delete y vs)) as Hdel.
+  { by intros [|y] ?; rewrite /= 1?delete_commute. }
+  induction e=> vs; simplify_map_eq; auto with f_equal.
+  - match goal with
+    | |- context [ <[?x:=_]> _ !! ?y ] =>
+       destruct (decide (x = y)); simplify_map_eq=> //
+    end. by case (vs !! _); simplify_option_eq.
+  - destruct (decide _) as [[??]|[<-%dec_stable|[<-%dec_stable ?]]%not_and_l_alt].
+    + rewrite !Hins // !Hdel. eauto with f_equal.
+    + by rewrite /= delete_insert_delete delete_idemp.
+    + by rewrite /= Hins // delete_insert_delete !Hdel delete_idemp.
+Qed.
+Lemma subst_map_binder_insert b v vs e :
+  subst_map (binder_insert b v vs) e =
+  subst' b v (subst_map (binder_delete b vs) e).
+Proof. destruct b; rewrite ?subst_map_insert //. Qed.
+
+(* subst_map on closed expressions *)
+Lemma subst_map_is_closed X e vs :
+  is_closed_expr X e →
+  (∀ x, x ∈ X → vs !! x = None) →
+  subst_map vs e = e.
+Proof.
+  revert X vs. assert (∀ x x1 x2 X (vs : gmap string val),
+    (∀ x, x ∈ X → vs !! x = None) →
+    x ∈ x2 :b: x1 :b: X →
+    binder_delete x1 (binder_delete x2 vs) !! x = None).
+  { intros x x1 x2 X vs ??. rewrite !lookup_binder_delete_None. set_solver. }
+  induction e=> X vs /= ? HX; repeat case_match; naive_solver eauto with f_equal.
+Qed.
+
+Lemma subst_map_is_closed_nil e vs : is_closed_expr [] e → subst_map vs e = e.
+Proof. intros. apply subst_map_is_closed with []; set_solver. Qed.
